\documentclass[12pt]{article}
\usepackage{amsmath}

\begin{document}
\section{Mathematical formula}
$$\cos \alpha=\frac{1}{2} \qquad \sin\beta =\frac{\sqrt{3}}{2} \qquad \tan  \theta =1$$
$$y^2=4 \qquad y=\pm 2$$
$$a^x+y \neq a^{x+y}$$
$$(a_1 +a_2)a_3=a_1 a_3+ a_2 a_3$$

\section{Integral operator}
$$\int x^2 \mathrm{d}x=\frac{x^3}{3}$$
$$\int_0 ^1 x^2 \mathrm{d}x=\frac{1}{3}$$
$$\int \frac{1}{x} \mathrm{d}x=\ln x$$
$$\iint_D (x^2+y^2)\mathrm{d}x\mathrm{d}y$$
$$\iiint(x^2+y^2+z^2)\mathrm{d}x\mathrm{d}y\mathrm{d}z$$
\newcommand{\md}{\mathrm{d}}
$$\int x^2 \md x=\frac{x^3}{3}$$
$$\iiint(x+y+z)\md x \md y \md z$$

\section{differential operator}
$$y' + p(x)y +q(x)=0$$

$$y'' + py' +qy=0$$

$$\frac{\md y}{\md x}=2x$$

$$\frac{\md ^2 y}{\md x^2} -x\frac{\md y}{\md x} +u=0$$

$$\frac{\partial u}{\partial t} + t\frac{\partial u}{\partial x}=0$$

$$\frac{\partial ^3 u}{\partial x^3}-6u\frac{\partial u}{\partial x} +\frac{\partial u}{\partial t}=0$$

\section{Sum operator}
$$\sum_{k=1} ^n k^2=\frac{1}{3} n^3 +\frac{1}{2} n^2 +\frac{1}{6} n$$

$$\lim _{n \to \infty} \sum_{k=1} ^n \frac{1}{k^2}=\frac{\pi ^2}{6}$$

\section{Array}
\begin{displaymath}
\left[\begin{array}{ccc}
1&2&3\\
4&5&6
\end{array}\right]
\end{displaymath}

\begin{displaymath}
\mathbf{H}_x=\frac{1}{3} \times \left[\begin{array}{ccc}
1&0&2\\
2&1&3\\
3&2&1
\end{array}\right]
\end{displaymath}

\begin{displaymath}
\left[\begin{array}{cccc}
1&2&\cdots &4\\
5&6&\cdots &7\\
\vdots &\vdots &\ddots &\vdots \\
8&9&\cdots &0
\end{array}\right]
\end{displaymath}

\begin{displaymath}
y=\left\{\begin{array}{ll}
a&d>1\\
b+x&d\leq 1
\end{array}\right.
\end{displaymath}

\section{eqnarray}
\begin{eqnarray}
\sin x &=& x-\frac{x^3}{3} +\frac{x^5}{5}- \frac{x^7}{7} +x-\frac{x^3}{3} +\frac{x^5}{5} \\ \nonumber
           & &\frac{x^7}{7} x-\frac{x^3}{3} +\frac{x^5}{5}- \frac{x^7}{7} +x+\frac{x^5}{5} +\cdots
\end{eqnarray}

\setlength\arraycolsep{2pt}
\begin{eqnarray}
A&=&(x-y)(x+y)\\ \nonumber
  &=&x^2-yx+xy-y^2\\ \nonumber
  &=&x^2-y^2 
\end{eqnarray}

\section{align}
\begin{align*}
A&=(x-y)(x+y)\\ \nonumber
  &=x^2-yx+xy-y^2\\ \nonumber
  &=x^2-y^2 
\end{align*}

\begin{align*}
f(x)&=\cos x \\
f'(x)&=-\sin x \\
f''(x)&=-cos x
\end{align*}

\end{document}